theories/lang_generic.v
@@ -1,11 +1,10 @@
-From gitrees Require Import prelude.
-From gitrees Require Import gitree.
+From gitrees Require Import prelude gitree utils.finite_sets.
 Require Import List.
 Import ListNotations.
 
 Require Import Binding.Lib Binding.Set.
 
-Section interp.
+Section ctx_interp.
   Local Open Scope type.
   Context {E: opsInterp}.
   Context {R} `{!Cofe R}.
@@ -25,6 +24,9 @@ Section interp.
   Next Obligation.
     solve_proper.
   Qed.
+
+  Program Definition ı_scope : interp_scope Empty_set
+    := λne (x : ∅), match x with end.
 
   Definition interp_scope_split {S1 S2 : Set} :
     interp_scope (sum S1 S2) -n> interp_scope S1 * interp_scope S2.
@@ -63,7 +65,7 @@ Section interp.
   Program Definition ren_scope {S S'} (δ : S [→] S') (env : interp_scope S')
     : interp_scope S := λne x, env (δ x).
 
-End interp.
+End ctx_interp.
 
 (* Common definitions and lemmas for Kripke logical relations *)
 Section kripke_logrel.
@@ -73,7 +75,7 @@ Section kripke_logrel.
   Variable rs : gReifiers a sz.
   Context {R} `{!Cofe R}.
 
-  Notation F := (gReifiers_ops a rs).
+  Notation F := (gReifiers_ops rs).
   Notation IT := (IT F R).
   Notation ITV := (ITV F R).
   Context `{!invGS Σ, !stateG rs R Σ}.
@@ -133,7 +135,7 @@ Section kripke_logrel_ctx_indep.
   Variable rs : gReifiers NotCtxDep sz.
   Context {R} `{!Cofe R}.
 
-  Notation F := (gReifiers_ops NotCtxDep rs).
+  Notation F := (gReifiers_ops rs).
   Notation IT := (IT F R).
   Notation ITV := (ITV F R).
   Context `{!invGS Σ, !stateG rs R Σ}.
@@ -165,3 +167,157 @@ Section kripke_logrel_ctx_indep.
 End kripke_logrel_ctx_indep.
 
 Arguments expr_pred_bind {_ _ _ _ _ _ _ _ _ _} f {_ _}.
+
+Section tm_interp.
+  Context {sz : nat} {a : is_ctx_dep}.
+  Variable rs : gReifiers a sz.
+  Context {R} `{!Cofe R}.
+
+  Notation F := (gReifiers_ops rs).
+  Notation IT := (IT F R).
+  Notation ITV := (ITV F R).
+  Context `{!invGS Σ, !stateG rs R Σ}.
+  Notation iProp := (iProp Σ).
+
+  Context {A : ofe}.
+  Variable (P : A -n> iProp).
+
+  Variable (ty : Set).
+  Variable (interp_ty : ty → (ITV -n> iProp)).
+  Variable (kripke : IT → (ITV -n> iProp) → iProp).
+
+  Definition ssubst_valid1 {S : Set}
+    (Γ : S -> ty)
+    (ss : interp_scope S) : iProp :=
+    (∀ x, □ kripke (ss x) (interp_ty (Γ x)))%I.
+
+  Global Instance ssubst_valid_pers `{∀ τ β, Persistent (interp_ty τ β)}
+    {S : Set} (Γ : S → ty) ss : Persistent (ssubst_valid1 Γ ss).
+  Proof. apply _. Qed.
+
+End tm_interp.
+
+Section tm_interp_fin.
+  Context {sz : nat} {a : is_ctx_dep}.
+  Variable rs : gReifiers a sz.
+  Context {R} `{!Cofe R}.
+
+  Notation F := (gReifiers_ops rs).
+  Notation IT := (IT F R).
+  Notation ITV := (ITV F R).
+  Context `{!invGS Σ, !stateG rs R Σ}.
+  Notation iProp := (iProp Σ).
+
+  Context {A : ofe}.
+  Variable (P : A -n> iProp).
+
+  Variable (ty : Set).
+  Variable (interp_ty : ty → (ITV -n> iProp)).
+  Variable (kripke : IT → (ITV -n> iProp) → iProp).
+
+  Program Definition ssubst_valid_fin1 {S : Set} `{!EqDecision S} `{!Finite S}
+    (Ω : S → ty) (ss : interp_scope S) : iProp
+    := ([∗ set] x ∈ (fin_to_set S),
+         (kripke (ss x) (interp_ty (Ω x)))%I).
+
+  Context (Q : iProp).
+
+  Definition valid_fin1 {S : Set} `{!EqDecision S} `{!Finite S} (Ω : S → ty)
+    (α : interp_scope S -n> IT) (τ : ty) : iProp :=
+    ∀ ss, Q
+          -∗ (ssubst_valid_fin1 Ω ss)
+          -∗ kripke (α ss) (interp_ty τ).
+
+  Lemma ssubst_valid_fin_empty1 (αs : interp_scope ∅) :
+    ⊢ ssubst_valid_fin1 □ αs.
+  Proof.
+    iStartProof.
+    unfold ssubst_valid_fin1.
+    rewrite fin_to_set_empty.
+    by iApply big_sepS_empty.
+  Qed.
+
+  Lemma ssubst_valid_fin_app1
+    {S1 S2 : Set} `{!EqDecision S1} `{!Finite S1}
+    `{!EqDecision S2} `{!Finite S2}
+    `{!EqDecision (S1 + S2)} `{!Finite (S1 + S2)}
+    (Ω1 : S1 → ty) (Ω2 : S2 → ty)
+    (αs : interp_scope (sum S1 S2)) :
+    (ssubst_valid_fin1 (sum_map' Ω1 Ω2) αs) ⊢
+    (ssubst_valid_fin1 Ω1 (interp_scope_split αs).1)
+    ∗ (ssubst_valid_fin1 Ω2 (interp_scope_split αs).2).
+  Proof.
+    iIntros "H".
+    rewrite /ssubst_valid_fin1 fin_to_set_sum big_sepS_union; first last.
+    {
+      apply elem_of_disjoint.
+      intros [x | x].
+      - rewrite !elem_of_list_to_set.
+        intros _ H2.
+        apply elem_of_list_fmap_2 in H2.
+        destruct H2 as [y [H2 H2']]; inversion H2.
+      - rewrite !elem_of_list_to_set.
+        intros H1 _.
+        apply elem_of_list_fmap_2 in H1.
+        destruct H1 as [y [H1 H1']]; inversion H1.
+    }
+    iDestruct "H" as "(H1 & H2)".
+    iSplitL "H1".
+    - rewrite big_opS_list_to_set; first last.
+      {
+        apply NoDup_fmap.
+        - intros ??; by inversion 1.
+        - apply NoDup_elements.
+      }
+      rewrite big_sepL_fmap /=.
+      rewrite big_sepS_elements.
+      iFrame "H1".
+    - rewrite big_opS_list_to_set; first last.
+      {
+        apply NoDup_fmap.
+        - intros ??; by inversion 1.
+        - apply NoDup_elements.
+      }
+      rewrite big_sepL_fmap /=.
+      rewrite big_sepS_elements.
+      iFrame "H2".
+  Qed.
+
+  Lemma ssubst_valid_fin_cons1 {S : Set} `{!EqDecision S} `{!Finite S}
+    (Ω : S → ty) (αs : interp_scope S) τ t :
+    ssubst_valid_fin1 Ω αs ∗ kripke t (interp_ty τ) ⊢ ssubst_valid_fin1 (Ω ▹ τ) (extend_scope αs t).
+  Proof.
+    iIntros "(H & G)".
+    rewrite /ssubst_valid_fin1.
+    rewrite fin_to_set_inc /=.
+    rewrite big_sepS_union; first last.
+    {
+      apply elem_of_disjoint.
+      intros [| x].
+      - rewrite !elem_of_list_to_set.
+        intros _ H2.
+        apply elem_of_list_fmap_2 in H2.
+        destruct H2 as [y [H2 H2']]; inversion H2.
+      - rewrite !elem_of_list_to_set.
+        intros H1 _.
+        apply elem_of_singleton_1 in H1.
+        inversion H1.
+    }
+    iSplitL "G".
+    - rewrite big_opS_singleton.
+      iFrame "G".
+    - erewrite big_opS_set_map.
+      + iFrame "H".
+      + intros ?? H; by inversion H.
+  Qed.
+
+  Lemma ssubst_valid_fin_lookup1 {S : Set} `{!EqDecision S} `{!Finite S}
+    (Ω : S → ty) (αs : interp_scope S) x :
+    ssubst_valid_fin1 Ω αs ⊢ kripke (αs x) (interp_ty (Ω x)).
+  Proof.
+    iIntros "H".
+    iDestruct (big_sepS_elem_of_acc _ _ x with "H") as "($ & _)";
+      first apply elem_of_fin_to_set.
+  Qed.
+
+End tm_interp_fin.
