theories/utils/finite_sets.v
@@ -1,0 +1,221 @@
+From stdpp Require Export finite gmap.
+Require Export Binding.Resolver Binding.Lib Binding.Set Binding.Auto Binding.Env.
+
+Lemma fin_to_set_sum {S1 S2 : Set} `{!EqDecision S1} `{!EqDecision S2}
+  `{!Finite S1} `{!Finite S2} `{HE : EqDecision (S1 + S2)} `{HF : @Finite (S1 + S2) HE}
+  : fin_to_set (S1 + S2)
+    = (set_map inl (fin_to_set S1 : gset S1))
+        ∪ (set_map inr (fin_to_set S2 : gset S2))
+      :> @gset (S1 + S2) HE (@finite_countable _ HE HF).
+Proof.
+  apply set_eq.
+  intros [x|x]; simpl; split; intros _.
+  - apply elem_of_union; left.
+    apply elem_of_map_2.
+    apply elem_of_fin_to_set.
+  - apply elem_of_fin_to_set.
+  - apply elem_of_union; right.
+    apply elem_of_map_2.
+    apply elem_of_fin_to_set.
+  - apply elem_of_fin_to_set.
+Qed.
+
+Lemma fin_to_set_empty `{HE : EqDecision ∅} `{HF : @Finite ∅ HE} :
+  fin_to_set ∅ = empty :> @gset ∅ HE (@finite_countable _ HE HF).
+Proof.
+  apply set_eq; intros [].
+Qed.
+
+Lemma fin_to_set_inc {S : Set} `{!EqDecision S} `{!Finite S}
+  `{HE : EqDecision (inc S)} `{HF : @Finite (inc S) HE}
+  : fin_to_set (inc S) = ({[VZ]} : gset (inc S)) ∪ (set_map VS (fin_to_set S : gset S))
+      :> @gset (inc S) HE (@finite_countable _ HE HF).
+Proof.
+  apply set_eq.
+  intros [| x].
+  - split.
+    + intros _; apply elem_of_union; left.
+      by apply elem_of_singleton.
+    + intros _; apply elem_of_fin_to_set.
+  - split.
+    + intros _; apply elem_of_union; right.
+      apply elem_of_map_2, elem_of_fin_to_set.
+    + intros H.
+      apply elem_of_fin_to_set.
+Qed.
+
+Section Sum.
+  (* Kenny Loggins starts playing in a background *)
+
+  Lemma EqDecisionLeft {S1 S2 : Set} {H : EqDecision (S1 + S2)} : EqDecision S1.
+  Proof.
+    intros x y.
+    destruct (decide (inl x = inl y)) as [G | G];
+      [left; by inversion G | right; intros C; by subst].
+  Qed.
+
+  Lemma EqDecisionRight {S1 S2 : Set} {H : EqDecision (S1 + S2)} : EqDecision S2.
+  Proof.
+    intros x y.
+    destruct (decide (inr x = inr y)) as [G | G];
+      [left; by inversion G | right; intros C; by subst].
+  Qed.
+
+  Lemma FiniteLeft {S1 S2 : Set} `{EqDecision S1}
+    `{EqDecision (S1 + S2)} `{Finite (S1 + S2)}
+    : Finite S1.
+  Proof.
+    unshelve econstructor.
+    - apply (foldr (λ x acc, match x with
+                             | inl x => x :: acc
+                             | inr _ => acc
+                             end) [] (enum (S1 + S2))).
+    - set (l := enum (S1 + S2)).
+      assert (NoDup l) as K; [apply (NoDup_enum (S1 + S2)) |].
+      clearbody l.
+      induction l as [| a l IH]; [constructor |].
+      destruct a as [a | a]; simpl.
+      + constructor.
+        * intros C.
+          assert (inl a ∈ l) as C'.
+          {
+            clear -C.
+            induction l as [| b l IH]; [inversion C |].
+            destruct b as [b | b]; simpl.
+            - rewrite foldr_cons in C.
+              rewrite elem_of_cons in C.
+              destruct C as [-> | C].
+              + apply elem_of_cons.
+                by left.
+              + right.
+                apply IH.
+                apply C.
+            - apply elem_of_cons.
+              right.
+              rewrite foldr_cons in C.
+              apply IH.
+              apply C.
+          }
+          by inversion K.
+        * apply IH.
+          by inversion K.
+      + apply IH.
+        by inversion K.
+    - intros x.
+      set (l := enum (S1 + S2)).
+      assert (inl x ∈ l) as K; [apply elem_of_enum |].
+      clearbody l.
+      induction l as [| a l IH]; [inversion K |].
+      destruct a as [a | a]; simpl.
+      + rewrite elem_of_cons in K.
+        destruct K as [K | K].
+        * inversion K; subst.
+          apply elem_of_cons; by left.
+        * apply elem_of_cons; right; by apply IH.
+      + rewrite elem_of_cons in K.
+        destruct K as [K | K]; [inversion K |].
+        by apply IH.
+  Qed.
+
+  Lemma FiniteRight {S1 S2 : Set} `{EqDecision S2}
+    `{EqDecision (S1 + S2)} `{H : Finite (S1 + S2)}
+    : Finite S2.
+  Proof.
+    unshelve econstructor.
+    - apply (foldr (λ x acc, match x with
+                             | inl _ => acc
+                             | inr x => x :: acc
+                             end) [] (enum (S1 + S2))).
+    - set (l := enum (S1 + S2)).
+      assert (NoDup l) as K; [apply NoDup_enum |].
+      clearbody l.
+      induction l as [| a l IH]; [constructor |].
+      destruct a as [a | a]; simpl.
+      + apply IH.
+        by inversion K.
+      + constructor.
+        * intros C.
+          assert (inr a ∈ l) as C'.
+          {
+            clear -C.
+            induction l as [| b l IH]; [inversion C |].
+            destruct b as [b | b]; simpl.
+            - apply elem_of_cons.
+              right.
+              rewrite foldr_cons in C.
+              apply IH, C.
+            - rewrite foldr_cons in C.
+              rewrite elem_of_cons in C.
+              destruct C as [-> | C].
+              + apply elem_of_cons.
+                by left.
+              + right.
+                apply IH, C.
+          }
+          by inversion K.
+        * apply IH.
+          by inversion K.
+    - intros x.
+      set (l := enum (S1 + S2)).
+      assert (inr x ∈ l) as K; [apply elem_of_enum |].
+      clearbody l.
+      induction l as [| a l IH]; [inversion K |].
+      destruct a as [a | a]; simpl.
+      + rewrite elem_of_cons in K.
+        destruct K as [K | K]; [inversion K |].
+        by apply IH.
+      + rewrite elem_of_cons in K.
+        destruct K as [K | K].
+        * inversion K; subst.
+          apply elem_of_cons; by left.
+        * apply elem_of_cons; right; by apply IH.
+  Qed.
+
+End Sum.
+
+Section Inc.
+  Context (S : Set).
+
+  Global Instance EqDecisionIncN {HS : EqDecision S} (n : nat) : EqDecision (Init.Nat.iter n inc S).
+  Proof using S.
+    induction n; simpl.
+    - apply _.
+    - intros [|x] [|y].
+      + by left.
+      + by right.
+      + by right.
+      + destruct (decide (x = y)) as [-> |]; [by left |].
+        right; by inversion 1.
+  Qed.
+
+  Global Instance EqDecisionInc {HS : EqDecision S} : EqDecision (inc S).
+  Proof using S.
+    assert (inc S = Init.Nat.iter 1 inc S) as ->; [done |].
+    by apply EqDecisionIncN.
+  Qed.
+
+  Global Instance FiniteIncN {HS : EqDecision S} (HF : Finite S) (n : nat) {HS' : EqDecision (Init.Nat.iter n inc S)} : Finite (Init.Nat.iter n inc S).
+  Proof using S.
+    induction n.
+    - apply (@surjective_finite S HS HF _ _ id).
+      apply _.
+    - simpl.
+      unshelve eapply (@surjective_finite (option (Init.Nat.iter n inc S))); simpl in *.
+      + intros [x |].
+        * apply (VS x).
+        * apply VZ.
+      + apply _.
+      + intros [| x]; simpl.
+        * exists None; reflexivity.
+        * exists (Some x); reflexivity.
+  Qed.
+
+  Global Instance FiniteInc {HS : EqDecision S} (HF : Finite S) (HE : EqDecision (inc S)) : Finite (inc S).
+  Proof using S.
+    assert (J : @Finite (Init.Nat.iter 1 inc S) HE).
+    { apply FiniteIncN, HF. }
+    simpl in J.
+    apply J.
+  Qed.
+
+End Inc.
